begin integration of kvservice

src/program_proof/tutorial/kvservice/proof.v
@@ -14,433 +14,433 @@ Unset Printing Projections.
 
 (********************************************************************************)
 
-Module putArgs.
-Record t :=
-  mk {
-      opId: u64 ;
-      key: string ;
-      val: string ;
-  }.
+(* Module putArgs. *)
+(* Record t := *)
+(*   mk { *)
+(*       opId: u64 ; *)
+(*       key: string ; *)
+(*       val: string ; *)
+(*   }. *)
 
-Definition encodes (x:list u8) (a:t) : Prop :=
-  x = u64_le a.(opId) ++ (u64_le $ length $ string_to_bytes a.(key)) ++
-      string_to_bytes a.(key) ++ string_to_bytes a.(val)
-.
+(* Definition encodes (x:list u8) (a:t) : Prop := *)
+(*   x = u64_le a.(opId) ++ (u64_le $ length $ string_to_bytes a.(key)) ++ *)
+(*       string_to_bytes a.(key) ++ string_to_bytes a.(val) *)
+(* . *)
 
-Section local_defs.
-Context `{!heapGS Σ}.
-Definition own (a:loc) (args:t) : iProp Σ :=
-  "HopId" ∷ a ↦[putArgs :: "opId"] #args.(opId) ∗
-  "Hkey" ∷ a ↦[putArgs :: "key"] #(str args.(key)) ∗
-  "Hval" ∷ a ↦[putArgs :: "val"] #(str args.(val))
-.
+(* Section local_defs. *)
+(* Context `{!heapGS Σ}. *)
+(* Definition own (a:loc) (args:t) : iProp Σ := *)
+(*   "HopId" ∷ a ↦[putArgs :: "opId"] #args.(opId) ∗ *)
+(*   "Hkey" ∷ a ↦[putArgs :: "key"] #(str args.(key)) ∗ *)
+(*   "Hval" ∷ a ↦[putArgs :: "val"] #(str args.(val)) *)
+(* . *)
 
-Lemma wp_encode args_ptr args :
-  {{{
-        own args_ptr args
-  }}}
-    encodePutArgs #args_ptr
-  {{{
-        (sl:Slice.t) enc_args, RET (slice_val sl); own args_ptr args ∗
-          ⌜encodes enc_args args⌝ ∗
-          own_slice sl byteT (DfracOwn 1) enc_args
-  }}}
-.
-Proof.
-  iIntros (Φ) "Hargs HΦ".
-  iNamed "Hargs".
-  wp_rec.
-  wp_apply wp_NewSlice.
-  iIntros (sl) "Hsl".
-  wp_apply wp_ref_to.
-  { done. }
-  iIntros (e) "He".
+(* Lemma wp_encode args_ptr args : *)
+(*   {{{ *)
+(*         own args_ptr args *)
+(*   }}} *)
+(*     encodePutArgs #args_ptr *)
+(*   {{{ *)
+(*         (sl:Slice.t) enc_args, RET (slice_val sl); own args_ptr args ∗ *)
+(*           ⌜encodes enc_args args⌝ ∗ *)
+(*           own_slice sl byteT (DfracOwn 1) enc_args *)
+(*   }}} *)
+(* . *)
+(* Proof. *)
+(*   iIntros (Φ) "Hargs HΦ". *)
+(*   iNamed "Hargs". *)
+(*   wp_rec. *)
+(*   wp_apply wp_NewSlice. *)
+(*   iIntros (sl) "Hsl". *)
+(*   wp_apply wp_ref_to. *)
+(*   { done. } *)
+(*   iIntros (e) "He". *)
 
-  wp_pures.
-  wp_loadField.
-  wp_load.
-  wp_apply (wp_WriteInt with "[$]").
-  iIntros (?) "Hsl".
-  rewrite replicate_0 /=.
-  wp_store.
+(*   wp_pures. *)
+(*   wp_loadField. *)
+(*   wp_load. *)
+(*   wp_apply (wp_WriteInt with "[$]"). *)
+(*   iIntros (?) "Hsl". *)
+(*   rewrite replicate_0 /=. *)
+(*   wp_store. *)
 
-  wp_loadField.
-  wp_apply wp_StringToBytes.
-  iIntros (key_sl) "Hkey_sl".
-  wp_pures.
+(*   wp_loadField. *)
+(*   wp_apply wp_StringToBytes. *)
+(*   iIntros (key_sl) "Hkey_sl". *)
+(*   wp_pures. *)
 
-  wp_apply wp_slice_len.
-  iDestruct (own_slice_sz with "Hkey_sl") as "%Hsz".
-  wp_load.
-  wp_apply (wp_WriteInt with "[$Hsl]").
-  iIntros (?) "Hsl".
-  wp_store.
+(*   wp_apply wp_slice_len. *)
+(*   iDestruct (own_slice_sz with "Hkey_sl") as "%Hsz". *)
+(*   wp_load. *)
+(*   wp_apply (wp_WriteInt with "[$Hsl]"). *)
+(*   iIntros (?) "Hsl". *)
+(*   wp_store. *)
 
-  wp_load.
-  iDestruct (own_slice_to_small with "Hkey_sl") as "Hkey_sl".
-  wp_apply (wp_WriteBytes with "[$Hsl $Hkey_sl]").
-  iIntros (?) "[Hsl Hkey_sl]".
-  wp_store.
+(*   wp_load. *)
+(*   iDestruct (own_slice_to_small with "Hkey_sl") as "Hkey_sl". *)
+(*   wp_apply (wp_WriteBytes with "[$Hsl $Hkey_sl]"). *)
+(*   iIntros (?) "[Hsl Hkey_sl]". *)
+(*   wp_store. *)
 
-  wp_loadField.
-  wp_apply (wp_StringToBytes).
-  iIntros (?) "Hval_sl".
-  iDestruct (own_slice_to_small with "Hval_sl") as "Hval_sl".
-  wp_load.
-  wp_apply (wp_WriteBytes with "[$Hsl $Hval_sl]").
-  iIntros (?) "[Hsl Hval_sl]".
-  wp_store.
+(*   wp_loadField. *)
+(*   wp_apply (wp_StringToBytes). *)
+(*   iIntros (?) "Hval_sl". *)
+(*   iDestruct (own_slice_to_small with "Hval_sl") as "Hval_sl". *)
+(*   wp_load. *)
+(*   wp_apply (wp_WriteBytes with "[$Hsl $Hval_sl]"). *)
+(*   iIntros (?) "[Hsl Hval_sl]". *)
+(*   wp_store. *)
 
-  wp_load.
-  iApply "HΦ".
-  iFrame.
-  iPureIntro.
-  unfold encodes.
-  repeat rewrite -assoc.
-  rewrite Hsz.
-  repeat f_equal.
-  word.
-Qed.
+(*   wp_load. *)
+(*   iApply "HΦ". *)
+(*   iFrame. *)
+(*   iPureIntro. *)
+(*   unfold encodes. *)
+(*   repeat rewrite -assoc. *)
+(*   rewrite Hsz. *)
+(*   repeat f_equal. *)
+(*   word. *)
+(* Qed. *)
 
-Lemma wp_decode  sl enc_args args q :
-  {{{
-        "%Henc" ∷ ⌜encodes enc_args args⌝ ∗
-        "Hsl" ∷ own_slice_small sl byteT q enc_args
-  }}}
-    decodePutArgs (slice_val sl)
-  {{{
-        (args_ptr:loc), RET #args_ptr; own args_ptr args
-  }}}
-.
-Proof.
-  iIntros (Φ) "Hpre HΦ".
-  iNamed "Hpre".
-  wp_rec.
-  wp_apply wp_ref_to.
-  { done. }
-  iIntros (e) "He".
-  wp_pures.
-  wp_apply wp_allocStruct.
-  { repeat econstructor. }
-  iIntros (args_ptr) "Hargs".
-  iDestruct (struct_fields_split with "Hargs") as "HH".
-  iNamed "HH".
+(* Lemma wp_decode  sl enc_args args q : *)
+(*   {{{ *)
+(*         "%Henc" ∷ ⌜encodes enc_args args⌝ ∗ *)
+(*         "Hsl" ∷ own_slice_small sl byteT q enc_args *)
+(*   }}} *)
+(*     decodePutArgs (slice_val sl) *)
+(*   {{{ *)
+(*         (args_ptr:loc), RET #args_ptr; own args_ptr args *)
+(*   }}} *)
+(* . *)
+(* Proof. *)
+(*   iIntros (Φ) "Hpre HΦ". *)
+(*   iNamed "Hpre". *)
+(*   wp_rec. *)
+(*   wp_apply wp_ref_to. *)
+(*   { done. } *)
+(*   iIntros (e) "He". *)
+(*   wp_pures. *)
+(*   wp_apply wp_allocStruct. *)
+(*   { repeat econstructor. } *)
+(*   iIntros (args_ptr) "Hargs". *)
+(*   iDestruct (struct_fields_split with "Hargs") as "HH". *)
+(*   iNamed "HH". *)
 
-  wp_pures.
-  wp_load.
-  rewrite Henc; clear dependent enc_args.
-  wp_apply (wp_ReadInt with "[$]").
-  iIntros (?) "Hsl".
-  wp_pures.
-  wp_storeField.
-  wp_store.
-  wp_load.
-  wp_apply (wp_ReadInt with "[$]").
-  iIntros (?) "Hsl".
-  wp_pures.
-  iDestruct (own_slice_small_sz with "Hsl") as %Hsz.
-  wp_apply (wp_ReadBytes with "[$]").
-  { rewrite length_app in Hsz. word. }
-  iIntros (??) "[Hkey Hval]".
-  wp_pures.
-  wp_apply (wp_StringFromBytes with "[$Hkey]").
-  iIntros "Hkey".
-  wp_storeField.
-  wp_apply (wp_StringFromBytes with "[$Hval]").
-  iIntros "Hval".
-  wp_storeField.
-  iModIntro.
-  iApply "HΦ".
-  do 2 rewrite string_to_bytes_to_string.
-  iFrame.
-Qed.
+(*   wp_pures. *)
+(*   wp_load. *)
+(*   rewrite Henc; clear dependent enc_args. *)
+(*   wp_apply (wp_ReadInt with "[$]"). *)
+(*   iIntros (?) "Hsl". *)
+(*   wp_pures. *)
+(*   wp_storeField. *)
+(*   wp_store. *)
+(*   wp_load. *)
+(*   wp_apply (wp_ReadInt with "[$]"). *)
+(*   iIntros (?) "Hsl". *)
+(*   wp_pures. *)
+(*   iDestruct (own_slice_small_sz with "Hsl") as %Hsz. *)
+(*   wp_apply (wp_ReadBytes with "[$]"). *)
+(*   { rewrite length_app in Hsz. word. } *)
+(*   iIntros (??) "[Hkey Hval]". *)
+(*   wp_pures. *)
+(*   wp_apply (wp_StringFromBytes with "[$Hkey]"). *)
+(*   iIntros "Hkey". *)
+(*   wp_storeField. *)
+(*   wp_apply (wp_StringFromBytes with "[$Hval]"). *)
+(*   iIntros "Hval". *)
+(*   wp_storeField. *)
+(*   iModIntro. *)
+(*   iApply "HΦ". *)
+(*   do 2 rewrite string_to_bytes_to_string. *)
+(*   iFrame. *)
+(* Qed. *)
 
-End local_defs.
-End putArgs.
+(* End local_defs. *)
+(* End putArgs. *)
 
-Module conditionalPutArgs.
-Record t :=
-  mk {
-      opId: u64 ;
-      key: string ;
-      expectedVal: string ;
-      newVal: string ;
-  }.
+(* Module conditionalPutArgs. *)
+(* Record t := *)
+(*   mk { *)
+(*       opId: u64 ; *)
+(*       key: string ; *)
+(*       expectedVal: string ; *)
+(*       newVal: string ; *)
+(*   }. *)
 
-Definition encodes (x:list u8) (a:t) : Prop :=
-  x = u64_le a.(opId) ++ (u64_le $ length $ string_to_bytes a.(key)) ++ string_to_bytes a.(key) ++
-      (u64_le $ length $ string_to_bytes a.(expectedVal)) ++ string_to_bytes a.(expectedVal) ++ string_to_bytes a.(newVal)
-.
+(* Definition encodes (x:list u8) (a:t) : Prop := *)
+(*   x = u64_le a.(opId) ++ (u64_le $ length $ string_to_bytes a.(key)) ++ string_to_bytes a.(key) ++ *)
+(*       (u64_le $ length $ string_to_bytes a.(expectedVal)) ++ string_to_bytes a.(expectedVal) ++ string_to_bytes a.(newVal) *)
+(* . *)
 
-Section local_defs.
-Context `{!heapGS Σ}.
-Definition own (a:loc) (args:t) : iProp Σ :=
-  "HopId" ∷ a ↦[conditionalPutArgs :: "opId"] #args.(opId) ∗
-  "Hkey" ∷ a ↦[conditionalPutArgs :: "key"] #(str args.(key)) ∗
-  "HexpectedVal" ∷ a ↦[conditionalPutArgs :: "expectedVal"] #(str args.(expectedVal)) ∗
-  "Hval" ∷ a ↦[conditionalPutArgs :: "newVal"] #(str args.(newVal))
-.
+(* Section local_defs. *)
+(* Context `{!heapGS Σ}. *)
+(* Definition own (a:loc) (args:t) : iProp Σ := *)
+(*   "HopId" ∷ a ↦[conditionalPutArgs :: "opId"] #args.(opId) ∗ *)
+(*   "Hkey" ∷ a ↦[conditionalPutArgs :: "key"] #(str args.(key)) ∗ *)
+(*   "HexpectedVal" ∷ a ↦[conditionalPutArgs :: "expectedVal"] #(str args.(expectedVal)) ∗ *)
+(*   "Hval" ∷ a ↦[conditionalPutArgs :: "newVal"] #(str args.(newVal)) *)
+(* . *)
 
-Lemma wp_encode args_ptr args :
-  {{{
-        own args_ptr args
-  }}}
-    encodeConditionalPutArgs #args_ptr
-  {{{
-        (sl:Slice.t) enc_args, RET (slice_val sl); own args_ptr args ∗
-          ⌜encodes enc_args args⌝ ∗
-          own_slice sl byteT (DfracOwn 1) enc_args
-  }}}
-.
-Proof.
-  iIntros (Φ) "Hargs HΦ".
-  iNamed "Hargs".
-  wp_rec.
-  wp_apply wp_NewSlice.
-  iIntros (sl) "Hsl".
-  wp_apply wp_ref_to.
-  { done. }
-  iIntros (e) "He".
-  wp_pures.
+(* Lemma wp_encode args_ptr args : *)
+(*   {{{ *)
+(*         own args_ptr args *)
+(*   }}} *)
+(*     encodeConditionalPutArgs #args_ptr *)
+(*   {{{ *)
+(*         (sl:Slice.t) enc_args, RET (slice_val sl); own args_ptr args ∗ *)
+(*           ⌜encodes enc_args args⌝ ∗ *)
+(*           own_slice sl byteT (DfracOwn 1) enc_args *)
+(*   }}} *)
+(* . *)
+(* Proof. *)
+(*   iIntros (Φ) "Hargs HΦ". *)
+(*   iNamed "Hargs". *)
+(*   wp_rec. *)
+(*   wp_apply wp_NewSlice. *)
+(*   iIntros (sl) "Hsl". *)
+(*   wp_apply wp_ref_to. *)
+(*   { done. } *)
+(*   iIntros (e) "He". *)
+(*   wp_pures. *)
 
-  wp_loadField.
-  wp_load.
-  wp_apply (wp_WriteInt with "[$]").
-  iIntros (?) "Hsl".
-  rewrite replicate_0 /=.
-  wp_store.
+(*   wp_loadField. *)
+(*   wp_load. *)
+(*   wp_apply (wp_WriteInt with "[$]"). *)
+(*   iIntros (?) "Hsl". *)
+(*   rewrite replicate_0 /=. *)
+(*   wp_store. *)
 
-  wp_loadField.
-  wp_apply wp_StringToBytes.
-  iIntros (key_sl) "Hkey_sl".
-  wp_pures.
-  wp_apply wp_slice_len.
-  iDestruct (own_slice_sz with "Hkey_sl") as "%Hsz".
-  wp_load.
-  wp_apply (wp_WriteInt with "[$Hsl]").
-  iIntros (?) "Hsl".
-  wp_store.
+(*   wp_loadField. *)
+(*   wp_apply wp_StringToBytes. *)
+(*   iIntros (key_sl) "Hkey_sl". *)
+(*   wp_pures. *)
+(*   wp_apply wp_slice_len. *)
+(*   iDestruct (own_slice_sz with "Hkey_sl") as "%Hsz". *)
+(*   wp_load. *)
+(*   wp_apply (wp_WriteInt with "[$Hsl]"). *)
+(*   iIntros (?) "Hsl". *)
+(*   wp_store. *)
 
-  wp_load.
-  iDestruct (own_slice_to_small with "Hkey_sl") as "Hkey_sl".
-  wp_apply (wp_WriteBytes with "[$Hsl $Hkey_sl]").
-  iIntros (?) "[Hsl Hkey_sl]".
-  wp_store.
+(*   wp_load. *)
+(*   iDestruct (own_slice_to_small with "Hkey_sl") as "Hkey_sl". *)
+(*   wp_apply (wp_WriteBytes with "[$Hsl $Hkey_sl]"). *)
+(*   iIntros (?) "[Hsl Hkey_sl]". *)
+(*   wp_store. *)
 
-  wp_loadField.
-  wp_apply (wp_StringToBytes).
-  iIntros (?) "Hexpect_sl".
-  iDestruct (own_slice_to_small with "Hexpect_sl") as "Hexpect_sl".
-  wp_pures.
+(*   wp_loadField. *)
+(*   wp_apply (wp_StringToBytes). *)
+(*   iIntros (?) "Hexpect_sl". *)
+(*   iDestruct (own_slice_to_small with "Hexpect_sl") as "Hexpect_sl". *)
+(*   wp_pures. *)
 
-  wp_apply wp_slice_len.
-  iDestruct (own_slice_small_sz with "Hexpect_sl") as %?.
-  wp_load.
-  wp_apply (wp_WriteInt with "[$Hsl]").
-  iIntros (?) "Hsl".
-  wp_store.
+(*   wp_apply wp_slice_len. *)
+(*   iDestruct (own_slice_small_sz with "Hexpect_sl") as %?. *)
+(*   wp_load. *)
+(*   wp_apply (wp_WriteInt with "[$Hsl]"). *)
+(*   iIntros (?) "Hsl". *)
+(*   wp_store. *)
 
-  wp_load.
-  wp_apply (wp_WriteBytes with "[$Hsl $Hexpect_sl]").
-  iIntros (?) "[Hsl Hexpect_sl]".
-  wp_store.
+(*   wp_load. *)
+(*   wp_apply (wp_WriteBytes with "[$Hsl $Hexpect_sl]"). *)
+(*   iIntros (?) "[Hsl Hexpect_sl]". *)
+(*   wp_store. *)
 
-  wp_loadField.
-  wp_apply (wp_StringToBytes).
-  iIntros (?) "Hval_sl".
-  wp_load.
-  iDestruct (own_slice_to_small with "Hval_sl") as "Hval_sl".
-  wp_apply (wp_WriteBytes with "[$Hsl $Hval_sl]").
-  iIntros (?) "[Hsl Hval_sl]".
-  wp_store.
+(*   wp_loadField. *)
+(*   wp_apply (wp_StringToBytes). *)
+(*   iIntros (?) "Hval_sl". *)
+(*   wp_load. *)
+(*   iDestruct (own_slice_to_small with "Hval_sl") as "Hval_sl". *)
+(*   wp_apply (wp_WriteBytes with "[$Hsl $Hval_sl]"). *)
+(*   iIntros (?) "[Hsl Hval_sl]". *)
+(*   wp_store. *)
 
-  wp_load.
-  iApply "HΦ".
-  iFrame.
-  iPureIntro.
-  unfold encodes.
-  repeat rewrite -assoc.
-  rewrite Hsz.
-  repeat f_equal; word.
-Qed.
+(*   wp_load. *)
+(*   iApply "HΦ". *)
+(*   iFrame. *)
+(*   iPureIntro. *)
+(*   unfold encodes. *)
+(*   repeat rewrite -assoc. *)
+(*   rewrite Hsz. *)
+(*   repeat f_equal; word. *)
+(* Qed. *)
 
-Lemma wp_decode  sl enc_args args q :
-  {{{
-        "%Henc" ∷ ⌜encodes enc_args args⌝ ∗
-        "Hsl" ∷ own_slice_small sl byteT q enc_args
-  }}}
-    decodeConditionalPutArgs (slice_val sl)
-  {{{
-        (args_ptr:loc), RET #args_ptr; own args_ptr args
-  }}}
-.
-Proof.
-  iIntros (Φ) "Hpre HΦ".
-  iNamed "Hpre".
-  wp_rec.
-  wp_apply wp_ref_to.
-  { done. }
-  iIntros (?) "He".
-  wp_pures.
-  wp_apply wp_allocStruct.
-  { repeat econstructor. }
-  iIntros (args_ptr) "Hargs".
-  wp_pures.
-  iDestruct (struct_fields_split with "Hargs") as "HH".
-  iNamed "HH".
-  wp_load.
-  rewrite Henc.
+(* Lemma wp_decode  sl enc_args args q : *)
+(*   {{{ *)
+(*         "%Henc" ∷ ⌜encodes enc_args args⌝ ∗ *)
+(*         "Hsl" ∷ own_slice_small sl byteT q enc_args *)
+(*   }}} *)
+(*     decodeConditionalPutArgs (slice_val sl) *)
+(*   {{{ *)
+(*         (args_ptr:loc), RET #args_ptr; own args_ptr args *)
+(*   }}} *)
+(* . *)
+(* Proof. *)
+(*   iIntros (Φ) "Hpre HΦ". *)
+(*   iNamed "Hpre". *)
+(*   wp_rec. *)
+(*   wp_apply wp_ref_to. *)
+(*   { done. } *)
+(*   iIntros (?) "He". *)
+(*   wp_pures. *)
+(*   wp_apply wp_allocStruct. *)
+(*   { repeat econstructor. } *)
+(*   iIntros (args_ptr) "Hargs". *)
+(*   wp_pures. *)
+(*   iDestruct (struct_fields_split with "Hargs") as "HH". *)
+(*   iNamed "HH". *)
+(*   wp_load. *)
+(*   rewrite Henc. *)
 
-  wp_apply (wp_ReadInt with "Hsl").
-  iIntros (?) "Hsl".
-  wp_pures.
-  wp_storeField.
-  wp_store.
+(*   wp_apply (wp_ReadInt with "Hsl"). *)
+(*   iIntros (?) "Hsl". *)
+(*   wp_pures. *)
+(*   wp_storeField. *)
+(*   wp_store. *)
 
-  wp_load.
-  wp_apply (wp_ReadInt with "Hsl").
-  iIntros (?) "Hsl".
-  wp_pures.
+(*   wp_load. *)
+(*   wp_apply (wp_ReadInt with "Hsl"). *)
+(*   iIntros (?) "Hsl". *)
+(*   wp_pures. *)
 
-  iDestruct (own_slice_small_sz with "Hsl") as %Hsz.
-  wp_apply (wp_ReadBytes with "[$Hsl]").
-  { rewrite length_app in Hsz. word. }
-  iIntros (??) "[Hkey Hsl]".
-  wp_pures.
-  wp_apply (wp_StringFromBytes with "[$Hkey]").
-  iIntros "_".
-  wp_storeField.
+(*   iDestruct (own_slice_small_sz with "Hsl") as %Hsz. *)
+(*   wp_apply (wp_ReadBytes with "[$Hsl]"). *)
+(*   { rewrite length_app in Hsz. word. } *)
+(*   iIntros (??) "[Hkey Hsl]". *)
+(*   wp_pures. *)
+(*   wp_apply (wp_StringFromBytes with "[$Hkey]"). *)
+(*   iIntros "_". *)
+(*   wp_storeField. *)
 
-  wp_apply (wp_ReadInt with "[$Hsl]").
-  iIntros (?) "Hsl".
-  wp_pures.
+(*   wp_apply (wp_ReadInt with "[$Hsl]"). *)
+(*   iIntros (?) "Hsl". *)
+(*   wp_pures. *)
 
-  wp_apply (wp_ReadBytes with "[$Hsl]").
-  { repeat rewrite length_app in Hsz. word. }
-  iIntros (??) "[Hexpect Hval]".
-  wp_pures.
+(*   wp_apply (wp_ReadBytes with "[$Hsl]"). *)
+(*   { repeat rewrite length_app in Hsz. word. } *)
+(*   iIntros (??) "[Hexpect Hval]". *)
+(*   wp_pures. *)
 
-  wp_apply (wp_StringFromBytes with "[$Hexpect]").
-  iIntros "_".
-  wp_storeField.
-  wp_apply (wp_StringFromBytes with "[$Hval]").
-  iIntros "_".
-  wp_storeField.
-  iModIntro. iApply "HΦ".
-  repeat rewrite string_to_bytes_to_string.
-  iFrame.
-Qed.
+(*   wp_apply (wp_StringFromBytes with "[$Hexpect]"). *)
+(*   iIntros "_". *)
+(*   wp_storeField. *)
+(*   wp_apply (wp_StringFromBytes with "[$Hval]"). *)
+(*   iIntros "_". *)
+(*   wp_storeField. *)
+(*   iModIntro. iApply "HΦ". *)
+(*   repeat rewrite string_to_bytes_to_string. *)
+(*   iFrame. *)
+(* Qed. *)
 
-End local_defs.
-End conditionalPutArgs.
+(* End local_defs. *)
+(* End conditionalPutArgs. *)
 
-Module getArgs.
-Record t :=
-  mk {
-      opId: u64 ;
-      key: string ;
-  }.
+(* Module getArgs. *)
+(* Record t := *)
+(*   mk { *)
+(*       opId: u64 ; *)
+(*       key: string ; *)
+(*   }. *)
 
-Definition encodes (x:list u8) (a:t) : Prop :=
-  x = u64_le a.(opId) ++ string_to_bytes a.(key)
-.
+(* Definition encodes (x:list u8) (a:t) : Prop := *)
+(*   x = u64_le a.(opId) ++ string_to_bytes a.(key) *)
+(* . *)
 
-Section local_defs.
-Context `{!heapGS Σ}.
-Definition own `{!heapGS Σ} (a:loc) (args:t) : iProp Σ :=
-  "HopId" ∷ a ↦[getArgs :: "opId"] #args.(opId) ∗
-  "Hkey" ∷ a ↦[getArgs :: "key"] #(str args.(key))
-.
+(* Section local_defs. *)
+(* Context `{!heapGS Σ}. *)
+(* Definition own `{!heapGS Σ} (a:loc) (args:t) : iProp Σ := *)
+(*   "HopId" ∷ a ↦[getArgs :: "opId"] #args.(opId) ∗ *)
+(*   "Hkey" ∷ a ↦[getArgs :: "key"] #(str args.(key)) *)
+(* . *)
 
-Lemma wp_encode args_ptr args :
-  {{{
-        own args_ptr args
-  }}}
-    encodeGetArgs #args_ptr
-  {{{
-        (sl:Slice.t) enc_args, RET (slice_val sl); own args_ptr args ∗
-          ⌜encodes enc_args args⌝ ∗
-          own_slice sl byteT (DfracOwn 1) enc_args
-  }}}
-.
-Proof.
-  iIntros (Φ) "Hargs HΦ".
-  iNamed "Hargs".
-  wp_rec.
-  wp_apply wp_NewSlice.
-  iIntros (?) "Hsl".
-  wp_apply (wp_ref_to).
-  { done. }
-  iIntros (?) "He".
-  wp_pures.
-  wp_loadField.
-  wp_load.
-  wp_apply (wp_WriteInt with "Hsl").
-  iIntros (?) "Hsl".
-  wp_store.
-  wp_loadField.
-  wp_apply (wp_StringToBytes).
-  iIntros (?) "Hkey_sl".
-  wp_load.
-  iDestruct (own_slice_to_small with "Hkey_sl") as "Hkey_sl".
-  wp_apply (wp_WriteBytes with "[$Hsl $Hkey_sl]").
-  iIntros (?) "[Hsl _]".
-  wp_store.
-  wp_load.
-  iModIntro. iApply "HΦ".
-  iFrame.
-  iPureIntro. done.
-Qed.
+(* Lemma wp_encode args_ptr args : *)
+(*   {{{ *)
+(*         own args_ptr args *)
+(*   }}} *)
+(*     encodeGetArgs #args_ptr *)
+(*   {{{ *)
+(*         (sl:Slice.t) enc_args, RET (slice_val sl); own args_ptr args ∗ *)
+(*           ⌜encodes enc_args args⌝ ∗ *)
+(*           own_slice sl byteT (DfracOwn 1) enc_args *)
+(*   }}} *)
+(* . *)
+(* Proof. *)
+(*   iIntros (Φ) "Hargs HΦ". *)
+(*   iNamed "Hargs". *)
+(*   wp_rec. *)
+(*   wp_apply wp_NewSlice. *)
+(*   iIntros (?) "Hsl". *)
+(*   wp_apply (wp_ref_to). *)
+(*   { done. } *)
+(*   iIntros (?) "He". *)
+(*   wp_pures. *)
+(*   wp_loadField. *)
+(*   wp_load. *)
+(*   wp_apply (wp_WriteInt with "Hsl"). *)
+(*   iIntros (?) "Hsl". *)
+(*   wp_store. *)
+(*   wp_loadField. *)
+(*   wp_apply (wp_StringToBytes). *)
+(*   iIntros (?) "Hkey_sl". *)
+(*   wp_load. *)
+(*   iDestruct (own_slice_to_small with "Hkey_sl") as "Hkey_sl". *)
+(*   wp_apply (wp_WriteBytes with "[$Hsl $Hkey_sl]"). *)
+(*   iIntros (?) "[Hsl _]". *)
+(*   wp_store. *)
+(*   wp_load. *)
+(*   iModIntro. iApply "HΦ". *)
+(*   iFrame. *)
+(*   iPureIntro. done. *)
+(* Qed. *)
 
-Lemma wp_decode  sl enc_args args q :
-  {{{
-        "%Henc" ∷ ⌜encodes enc_args args⌝ ∗
-        "Hsl" ∷ own_slice_small sl byteT q enc_args
-  }}}
-    decodeGetArgs (slice_val sl)
-  {{{
-        (args_ptr:loc), RET #args_ptr; own args_ptr args
-  }}}
-.
-Proof.
-  iIntros (Φ) "Hpre HΦ".
-  iNamed "Hpre".
-  wp_rec.
-  wp_apply (wp_ref_to).
-  { done. }
-  iIntros (?) "He".
-  wp_pures.
-  wp_apply (wp_ref_of_zero).
-  { done. }
-  iIntros (?) "HkeyBytes".
-  wp_pures.
-  wp_apply wp_allocStruct.
-  { repeat econstructor. }
-  iIntros (args_ptr) "Hargs".
-  iDestruct (struct_fields_split with "Hargs") as "HH".
-  iNamed "HH".
-  wp_pures.
-  wp_load.
-  rewrite Henc.
-  wp_apply (wp_ReadInt with "[$Hsl]").
-  iIntros (?) "Hsl".
-  wp_pures.
-  wp_storeField.
-  wp_store.
+(* Lemma wp_decode  sl enc_args args q : *)
+(*   {{{ *)
+(*         "%Henc" ∷ ⌜encodes enc_args args⌝ ∗ *)
+(*         "Hsl" ∷ own_slice_small sl byteT q enc_args *)
+(*   }}} *)
+(*     decodeGetArgs (slice_val sl) *)
+(*   {{{ *)
+(*         (args_ptr:loc), RET #args_ptr; own args_ptr args *)
+(*   }}} *)
+(* . *)
+(* Proof. *)
+(*   iIntros (Φ) "Hpre HΦ". *)
+(*   iNamed "Hpre". *)
+(*   wp_rec. *)
+(*   wp_apply (wp_ref_to). *)
+(*   { done. } *)
+(*   iIntros (?) "He". *)
+(*   wp_pures. *)
+(*   wp_apply (wp_ref_of_zero). *)
+(*   { done. } *)
+(*   iIntros (?) "HkeyBytes". *)
+(*   wp_pures. *)
+(*   wp_apply wp_allocStruct. *)
+(*   { repeat econstructor. } *)
+(*   iIntros (args_ptr) "Hargs". *)
+(*   iDestruct (struct_fields_split with "Hargs") as "HH". *)
+(*   iNamed "HH". *)
+(*   wp_pures. *)
+(*   wp_load. *)
+(*   rewrite Henc. *)
+(*   wp_apply (wp_ReadInt with "[$Hsl]"). *)
+(*   iIntros (?) "Hsl". *)
+(*   wp_pures. *)
+(*   wp_storeField. *)
+(*   wp_store. *)
 
-  wp_load.
-  wp_apply (wp_StringFromBytes with "[$Hsl]").
-  iIntros "_".
-  wp_storeField.
-  iModIntro.
-  iApply "HΦ".
-  repeat rewrite string_to_bytes_to_string.
-  iFrame.
-Qed.
+(*   wp_load. *)
+(*   wp_apply (wp_StringFromBytes with "[$Hsl]"). *)
+(*   iIntros "_". *)
+(*   wp_storeField. *)
+(*   iModIntro. *)
+(*   iApply "HΦ". *)
+(*   repeat rewrite string_to_bytes_to_string. *)
+(*   iFrame. *)
+(* Qed. *)
 
-End local_defs.
+(* End local_defs. *)
 
-End getArgs.
+(* End getArgs. *)
 
 (********************************************************************************)
 
@@ -541,21 +541,21 @@ Definition getFreshNum_core_spec (Φ:u64 → iPropO Σ): iPropO Σ :=
 Global Instance getFreshNum_core_MonotonicPred : MonotonicPred (getFreshNum_core_spec).
 Proof. apply _. Qed.
 
-Definition put_core_spec (args:putArgs.t) (Φ:unit → iPropO Σ): iPropO Σ :=
+Definition put_core_spec (args:put.C) (Φ:unit → iPropO Σ): iPropO Σ :=
   (* TUTORIAL: write a more useful spec *)
   Φ ().
 
 Global Instance put_core_MonotonicPred args : MonotonicPred (put_core_spec args).
 Proof. apply _. Qed.
 
-Definition conditionalPut_core_spec (args:conditionalPutArgs.t) (Φ:string → iPropO Σ): iPropO Σ :=
+Definition conditionalPut_core_spec (args:conditionalPut.C) (Φ:string → iPropO Σ): iPropO Σ :=
   (* TUTORIAL: write a more useful spec *)
   (∀ status, Φ status)%I.
 
 Global Instance conditionalPut_core_MonotonicPred args : MonotonicPred (conditionalPut_core_spec args).
 Proof. apply _. Qed.
 
-Definition get_core_spec (args:getArgs.t) (Φ:string → iPropO Σ): iPropO Σ :=
+Definition get_core_spec (args:get.C) (Φ:string → iPropO Σ): iPropO Σ :=
   (* TUTORIAL: write a more useful spec *)
   (∀ ret, Φ ret)%I.
 
@@ -609,11 +609,11 @@ Proof.
   iApply "Hspec".
 Qed.
 
-Lemma wp_Server__put (s:loc) args_ptr (args:putArgs.t) Ψ :
+Lemma wp_Server__put (s:loc) args_ptr (args:put.C) Ψ :
   {{{
         "#Hsrv" ∷ is_Server s ∗
         "Hspec" ∷ put_core_spec args Ψ ∗
-        "Hargs" ∷ putArgs.own args_ptr args
+        "Hargs" ∷ put.own args_ptr args (DfracOwn 1)
   }}}
   Server__put #s #args_ptr
   {{{
@@ -627,9 +627,6 @@ Proof.
   wp_apply (wp_Mutex__Lock with "[$]") as "[Hlocked Hown]"; iNamed "Hown".
   iNamed "Hargs".
   wp_auto.
-
-  wp_loadField.
-
   wp_apply (wp_MapGet with "HlastRepliesM") as (??) "[%HlastReply HlastRepliesM]".
   wp_if_destruct; wp_auto.
   { (* case: this is a duplicate request *)
@@ -654,11 +651,11 @@ Proof.
   iApply ("HΦ" with "Hspec").
 Qed.
 
-Lemma wp_Server__conditionalPut (s:loc) args_ptr (args:conditionalPutArgs.t) Ψ :
+Lemma wp_Server__conditionalPut (s:loc) args_ptr (args:conditionalPut.C) Ψ :
   {{{
         "#Hsrv" ∷ is_Server s ∗
         "Hspec" ∷ conditionalPut_core_spec args Ψ ∗
-        "Hargs" ∷ conditionalPutArgs.own args_ptr args
+        "Hargs" ∷ conditionalPut.own args_ptr args (DfracOwn 1)
   }}}
     Server__conditionalPut #s #args_ptr
   {{{ r, RET #(str r); Ψ r }}}
@@ -714,11 +711,11 @@ Proof.
   iApply ("HΦ" with "Hspec").
 Qed.
 
-Lemma wp_Server__get (s:loc) args_ptr (args:getArgs.t) Ψ :
+Lemma wp_Server__get (s:loc) args_ptr (args:get.C) Ψ :
   {{{
         "#Hsrv" ∷ is_Server s ∗
         "Hspec" ∷ get_core_spec args Ψ ∗
-        "Hargs" ∷ getArgs.own args_ptr args
+        "Hargs" ∷ get.own args_ptr args (DfracOwn 1)
   }}}
     Server__get #s #args_ptr
   {{{
@@ -813,7 +810,7 @@ Defined.
 Program Definition put_spec :=
   λ (enc_args:list u8), λne (Φ : list u8 -d> iPropO Σ) ,
   (∃ args,
-   "%Henc" ∷ ⌜putArgs.encodes enc_args args⌝ ∗
+   "%Henc" ∷ ⌜put.has_encoding enc_args args⌝ ∗
    put_core_spec args (λ _, ∀ enc_reply, Φ enc_reply)
   )%I
 .
@@ -824,7 +821,7 @@ Defined.
 Program Definition conditionalPut_spec :=
   λ (enc_args:list u8), λne (Φ : list u8 -d> iPropO Σ) ,
   (∃ args,
-   "%Henc" ∷ ⌜conditionalPutArgs.encodes enc_args args⌝ ∗
+   "%Henc" ∷ ⌜conditionalPut.has_encoding enc_args args⌝ ∗
    conditionalPut_core_spec args (λ rep, Φ (string_to_bytes rep))
   )%I
 .
@@ -835,7 +832,7 @@ Defined.
 Program Definition get_spec :=
   λ (enc_args:list u8), λne (Φ : list u8 -d> iPropO Σ) ,
   (∃ args,
-   "%Henc" ∷ ⌜getArgs.encodes enc_args args⌝ ∗
+   "%Henc" ∷ ⌜get.has_encoding enc_args args⌝ ∗
    get_core_spec args (λ rep, Φ (string_to_bytes rep))
   )%I
 .
@@ -924,9 +921,9 @@ Proof.
       iIntros (?????) "!# (Hreq_sl & Hrep & Hspec) HΦ".
       wp_pures.
       iDestruct "Hspec" as (?) "[%Henc Hspec]".
-      wp_apply (getArgs.wp_decode with "[$Hreq_sl]").
-      { by iPureIntro. }
-      iIntros (?) "[Hargs Hreq_sl]".
+      wp_apply (get.wp_Decode _ _ _ [] with "[Hreq_sl]").
+      { rewrite app_nil_r. iFrame. by iPureIntro. }
+      iIntros (??) "[Hargs Hreq_sl]".
       wp_apply (wp_Server__get with "[$]").
       iIntros (?) "HΨ".
       wp_pures. wp_apply wp_StringToBytes.
@@ -943,9 +940,9 @@ Proof.
       iIntros (?????) "!# (Hreq_sl & Hrep & Hspec) HΦ".
       wp_pures.
       iDestruct "Hspec" as (?) "[%Henc Hspec]".
-      wp_apply (conditionalPutArgs.wp_decode with "[$Hreq_sl]").
-      { done. }
-      iIntros (?) "[Hargs Hreq_sl]".
+      wp_apply (conditionalPut.wp_Decode _ _ _ [] with "[Hreq_sl]").
+      { rewrite app_nil_r. iFrame. done. }
+      iIntros (??) "[Hargs Hreq_sl]".
       wp_apply (wp_Server__conditionalPut with "[$]").
       iIntros (?) "HΨ".
       wp_apply wp_StringToBytes.
@@ -962,9 +959,9 @@ Proof.
       iIntros (?????) "!# (Hreq_sl & Hrep & Hspec) HΦ".
       wp_pures.
       iDestruct "Hspec" as (?) "[%Henc Hspec]".
-      wp_apply (putArgs.wp_decode with "[$Hreq_sl]").
-      { done. }
-      iIntros (?) "Hargs".
+      wp_apply (put.wp_Decode _ _ _ [] with "[Hreq_sl]").
+      { rewrite app_nil_r. iFrame. done. }
+      iIntros (??) "Hargs". iDestruct "Hargs" as "[Hargs _]".
       wp_apply (wp_Server__put with "[$Hsrv $Hargs Hspec //]").
       iIntros "HΨ". wp_pures.
       iApply "HΦ"; iFrame.
@@ -1091,7 +1088,7 @@ Qed.
 
 Lemma wp_Client__putRpc Post cl args args_ptr :
   {{{
-        "Hargs" ∷ putArgs.own args_ptr args ∗
+        "Hargs" ∷ put.own args_ptr args DfracDiscarded ∗
         "#Hcl" ∷ is_Client cl ∗
         "#Hspec" ∷ □ put_core_spec args Post
   }}}
@@ -1109,8 +1106,9 @@ Proof.
   { done. }
   iIntros (rep_ptr) "Hrep".
   wp_pures.
-  wp_apply (putArgs.wp_encode with "[$]").
-  iIntros (??) "(Hargs & %Henc & Hreq_sl)".
+  wp_apply wp_NewSlice. iIntros (s) "Hs".
+  wp_apply (put.wp_Encode with "[$]").
+  iIntros (??) "(%Henc & Hreq_sl)".
   wp_pures.
   iNamed "Hcl".
   wp_loadField.
@@ -1149,7 +1147,7 @@ Qed.
 
 Lemma wp_Client__conditionalPutRpc Post cl args args_ptr :
   {{{
-        "Hargs" ∷ conditionalPutArgs.own args_ptr args ∗
+        "Hargs" ∷ conditionalPut.own args_ptr args DfracDiscarded ∗
         "#Hcl" ∷ is_Client cl ∗
         "#Hspec" ∷ □ conditionalPut_core_spec args Post
   }}}
@@ -1167,8 +1165,9 @@ Proof.
   { done. }
   iIntros (rep_ptr) "Hrep".
   wp_pures.
-  wp_apply (conditionalPutArgs.wp_encode with "[$]").
-  iIntros (??) "(Hargs & %Henc & Hreq_sl)".
+  wp_apply wp_NewSlice. iIntros (s) "Hs".
+  wp_apply (conditionalPut.wp_Encode with "[$]").
+  iIntros (??) "(%Henc & Hreq_sl)".
   wp_pures.
   iNamed "Hcl".
   wp_loadField.
@@ -1212,7 +1211,7 @@ Qed.
 
 Lemma wp_Client__getRpc Post cl args args_ptr :
   {{{
-        "Hargs" ∷ getArgs.own args_ptr args ∗
+        "Hargs" ∷ get.own args_ptr args DfracDiscarded ∗
         "#Hcl" ∷ is_Client cl ∗
         "#Hspec" ∷ □ get_core_spec args Post
   }}}
@@ -1230,8 +1229,9 @@ Proof.
   { done. }
   iIntros (rep_ptr) "Hrep".
   wp_pures.
-  wp_apply (getArgs.wp_encode with "[$]").
-  iIntros (??) "(Hargs & %Henc & Hreq_sl)".
+  wp_apply wp_NewSlice. iIntros (s) "Hs".
+  wp_apply (get.wp_Encode with "[$]").
+  iIntros (??) "(%Henc & Hreq_sl)".
   wp_pures.
   iNamed "Hcl".
   wp_loadField.
@@ -1343,8 +1343,8 @@ Proof.
   wp_loadField.
 
   (* TUTORIAL: *)
-  wp_apply (wp_Client__putRpc (λ _, True)%I with "[Hcl opId key val]").
-  { instantiate (2:=putArgs.mk _ _ _). iFrame "∗#". done. }
+  wp_apply (wp_Client__putRpc (λ _, True)%I with "[Hcl OpId Key Val]").
+  { instantiate (2:=put.mkC _ _ _). iFrame "∗#". done. }
   iClear "Hpost".
   iIntros (err) "Hpost".
   wp_pures.
