flake.nix
@@ -17,8 +17,8 @@
         src = pkgs.fetchFromGitHub {
           owner = "mjschwenne";
           repo = "grackle";
-          rev = "967767505d688aa2c578d75653e3cbd96af7a5bd";
-          hash = "sha256-z9hl6fjFZH8t3DtvGVedMJDg1fL6+8XyANBsH3DE4r8=";
+          rev = "ee753e57e3ad574d7d3f76f7de97af8817ac184c";
+          sha256 = "0j532jnk52sfk36spkl7knd6ryqwg19ih5sg6pb9f2qy9lsyaw9g";
         };
         vendorHash = "sha256-Wk2v0HSAkrzxHJvCfbw6xOn0OQ1xukvYjDxk3c2LmH8=";
         checkPhase = false;
@@ -29,7 +29,7 @@
           owner = "goose-lang";
           repo = "goose";
           rev = "585abc3cfef50dd466e112d7c535dbdfccd3c0ca";
-          hash = "sha256-M4zaZ1DdecYXeDugrL+TV7HWPMLuj1P25G6mf+fgljg=";
+          sha256 = "sha256-M4zaZ1DdecYXeDugrL+TV7HWPMLuj1P25G6mf+fgljg=";
         };
         vendorHash = "sha256-HCJ8v3TSv4UrkOsRuENWVz5Z7zQ1UsOygx0Mo7MELzY=";
       };
